PARM ptoa: WIP
Signed-off-by: Kyeongmin Cho <kyeongmin.cho@kaist.ac.kr>

src/equiv/PFtoA1.v
@@ -27,16 +27,16 @@ Set Implicit Arguments.
 
 Inductive sim_trace (p: program) (mem: Memory.t) (tid: Id.t):
   forall (tr: list (ExecUnit.t (A:=unit))) (atr: list AExecUnit.t)
-     (wl: list (nat -> option (Loc.t * Time.t))) (rl: list (nat -> option (Loc.t * Time.t)))
+     (wl: list (nat -> option (Loc.t * Time.t))) (rl: list (nat -> option (Loc.t * Time.t))) (fl: list (nat -> option (Loc.t * Time.t)))
      (cov: list (nat -> Time.t)) (vext: list (nat -> Time.t)), Prop :=
 | sim_trace_init
     st lc stmts
     (FIND: IdMap.find tid (Machine.init_with_promises p mem).(Machine.tpool) = Some (st, lc))
     (STMT: IdMap.find tid p = Some stmts):
     sim_trace p mem tid [ExecUnit.mk st lc mem] [AExecUnit.mk (State.init stmts) ALocal.init]
-              [fun _ => None] [fun _ => None] [fun _ => Time.bot] [fun _ => Time.bot]
+              [fun _ => None] [fun _ => None] [fun _ => None] [fun _ => Time.bot] [fun _ => Time.bot]
 | sim_trace_step
-    e ae tr eu1 eu2 atr aeu1 aeu2 rl r1 r2 wl w1 w2 covl cov1 cov2 vextl vext1 vext2
+    e ae tr eu1 eu2 atr aeu1 aeu2 rl r1 r2 wl w1 w2 fl f1 f2 covl cov1 cov2 vextl vext1 vext2
     (STEP: ExecUnit.state_step0 tid e e eu1 eu2)
     (ASTATE_STEP: State.step ae aeu1.(AExecUnit.state) aeu2.(AExecUnit.state))
     (ALOCAL_STEP: ALocal.step ae aeu1.(AExecUnit.local) aeu2.(AExecUnit.local))
@@ -65,6 +65,17 @@ Inductive sim_trace (p: program) (mem: Memory.t) (tid: Id.t):
                             else r1 eid)
                | _ => r1
                end)
+    (F: f2 = match e with
+               | Event.flushopt vloc =>
+                 (fun eid => if Nat.eqb eid (ALocal.next_eid aeu1.(AExecUnit.local))
+                            then Some (vloc.(ValA.val),
+                                       Memory.latest_ts
+                                         vloc.(ValA.val)
+                                         (eu2.(ExecUnit.local).(Local.lper) vloc.(ValA.val)).(View.ts)
+                                         mem)
+                            else f1 eid)
+               | _ => f1
+               end)
     (COV: cov2 = match e with
                  | Event.read _ _ _ vloc _
                  | Event.write _ _ vloc _ (ValA.mk _ 0 _) =>
@@ -74,6 +85,13 @@ Inductive sim_trace (p: program) (mem: Memory.t) (tid: Id.t):
                                      (eu2.(ExecUnit.local).(Local.coh) vloc.(ValA.val)).(View.ts)
                                      mem
                               else cov1 eid)
+                 | Event.flushopt vloc =>
+                   (fun eid => if Nat.eqb eid (ALocal.next_eid aeu1.(AExecUnit.local))
+                               then Memory.latest_ts
+                                      vloc.(ValA.val)
+                                      (eu2.(ExecUnit.local).(Local.lper) vloc.(ValA.val)).(View.ts)
+                                      mem
+                               else cov1 eid)
                  | _ => cov1
                  end)
     (VEXT: vext2 = match e with
@@ -85,10 +103,14 @@ Inductive sim_trace (p: program) (mem: Memory.t) (tid: Id.t):
                      (fun eid => if Nat.eqb eid (ALocal.next_eid aeu1.(AExecUnit.local))
                                 then (eu2.(ExecUnit.local).(Local.coh) vloc.(ValA.val)).(View.ts)
                                 else vext1 eid)
+                   | Event.flushopt vloc =>
+                     (fun eid => if Nat.eqb eid (ALocal.next_eid aeu1.(AExecUnit.local))
+                                 then (eu2.(ExecUnit.local).(Local.lper) vloc.(ValA.val)).(View.ts)
+                                 else vext1 eid)
                    | _ => vext1
                    end)
-    (TRACE: sim_trace p mem tid (eu1::tr) (aeu1::atr) (w1::wl) (r1::rl) (cov1::covl) (vext1::vextl)):
-    sim_trace p mem tid (eu2::eu1::tr) (aeu2::aeu1::atr) (w2::w1::wl) (r2::r1::rl) (cov2::cov1::covl) (vext2::vext1::vextl)
+    (TRACE: sim_trace p mem tid (eu1::tr) (aeu1::atr) (w1::wl) (r1::rl) (f1::fl) (cov1::covl) (vext1::vextl)):
+    sim_trace p mem tid (eu2::eu1::tr) (aeu2::aeu1::atr) (w2::w1::wl) (r2::r1::rl) (f2::f1::fl) (cov2::cov1::covl) (vext2::vext1::vextl)
 .
 
 Definition sim_traces
@@ -97,19 +119,21 @@ Definition sim_traces
            (atrs: IdMap.t (list AExecUnit.t))
            (ws: IdMap.t (list (nat -> option (Loc.t * Time.t))))
            (rs: IdMap.t (list (nat -> option (Loc.t * Time.t))))
+            (fs: IdMap.t (list (nat -> option (Loc.t * Time.t))))
            (covs: IdMap.t (list (nat -> Time.t)))
            (vexts: IdMap.t (list (nat -> Time.t)))
   : Prop :=
-  IdMap.Forall6 (sim_trace p mem) trs atrs ws rs covs vexts.
+  IdMap.Forall7 (sim_trace p mem) trs atrs ws rs fs covs vexts.
 
 Lemma sim_trace_last
-      p mem tid tr atr wl rl covl vextl
-      (SIM: sim_trace p mem tid tr atr wl rl covl vextl):
-  exists eu tr' aeu atr' w wl' r rl' cov covl' vext vextl',
+      p mem tid tr atr wl rl fl covl vextl
+      (SIM: sim_trace p mem tid tr atr wl rl fl covl vextl):
+  exists eu tr' aeu atr' w wl' r rl' f fl' cov covl' vext vextl',
     <<HDTR: tr = eu :: tr'>> /\
     <<HDATR: atr = aeu :: atr'>> /\
     <<HDWL: wl = w :: wl'>> /\
     <<HDRL: rl = r :: rl'>> /\
+    <<HDFL: fl = f :: fl'>> /\
     <<HDCOVL: covl = cov :: covl'>> /\
     <<HDVEXTL: vextl = vext :: vextl'>>.
 Proof.
@@ -117,11 +141,12 @@ Proof.
 Qed.
 
 Lemma sim_trace_length
-      p mem tid tr atr wl rl covl vextl
-      (SIM: sim_trace p mem tid tr atr wl rl covl vextl):
+      p mem tid tr atr wl rl fl covl vextl
+      (SIM: sim_trace p mem tid tr atr wl rl fl covl vextl):
   <<LENGTH_ATR: List.length atr = List.length tr>> /\
   <<LENGTH_WL: List.length wl = List.length tr>> /\
   <<LENGTH_RL: List.length rl = List.length tr>> /\
+  <<LENGTH_FL: List.length fl = List.length tr>> /\
   <<LENGTH_COVL: List.length covl = List.length tr>> /\
   <<LENGTH_VEXTL: List.length vextl = List.length tr>>.
 Proof.
@@ -129,9 +154,9 @@ Proof.
 Qed.
 
 Lemma sim_trace_memory
-      p mem tid tr atr rl wl covl vextl
+      p mem tid tr atr rl wl fl covl vextl
       eu tr'
-      (SIM: sim_trace p mem tid tr atr rl wl covl vextl)
+      (SIM: sim_trace p mem tid tr atr wl rl fl covl vextl)
       (EU: tr = eu :: tr'):
   mem = eu.(ExecUnit.mem).
 Proof.
@@ -143,11 +168,11 @@ Proof.
 Qed.
 
 Lemma sim_traces_memory
-      p trs atrs rs ws covs vexts
+      p trs atrs rs ws fs covs vexts
       m
       ts loc val tid
       (STEP: Machine.pf_exec p m)
-      (SIM: sim_traces p m.(Machine.mem) trs atrs ws rs covs vexts)
+      (SIM: sim_traces p m.(Machine.mem) trs atrs ws rs fs covs vexts)
       (TR: IdMap.Forall2
              (fun tid tr sl => exists l, tr = (ExecUnit.mk (fst sl) (snd sl) m.(Machine.mem)) :: l)
              trs m.(Machine.tpool))
@@ -304,8 +329,8 @@ Qed.
 Lemma promising_pf_sim_traces
       p m
       (STEP: Machine.pf_exec p m):
-  exists trs atrs ws rs covs vexts ex (PRE: Valid.pre_ex p ex),
-    <<SIM: sim_traces p m.(Machine.mem) trs atrs ws rs covs vexts>> /\
+  exists trs atrs ws rs fs covs vexts ex (PRE: Valid.pre_ex p ex),
+    <<SIM: sim_traces p m.(Machine.mem) trs atrs ws rs fs covs vexts>> /\
     <<TR: IdMap.Forall2
             (fun tid tr sl => exists l, tr = (ExecUnit.mk (fst sl) (snd sl) m.(Machine.mem)) :: l)
             trs m.(Machine.tpool)>> /\
@@ -315,8 +340,8 @@ Lemma promising_pf_sim_traces
 Proof.
   inv STEP. exploit state_exec_rtc_state_step; eauto. i. des.
   eapply Machine.equiv_no_promise in NOPROMISE; eauto. revert NOPROMISE.
-  cut (exists trs atrs ws rs covs vexts ex (PRE: Valid.pre_ex p ex),
-    <<SIM: sim_traces p (Machine.mem m2') trs atrs ws rs covs vexts>> /\
+  cut (exists trs atrs ws rs fs covs vexts ex (PRE: Valid.pre_ex p ex),
+    <<SIM: sim_traces p (Machine.mem m2') trs atrs ws rs fs covs vexts>> /\
     <<TR: forall tid, opt_rel
             (fun tr sl => exists l, tr = (ExecUnit.mk (fst sl) (snd sl) (Machine.mem m2')) :: l)
             (IdMap.find tid trs)
@@ -331,9 +356,10 @@ Proof.
     eexists (IdMap.map (fun x => [x]) (IdMap.mapi (fun _ _ => _) p)).
     eexists (IdMap.mapi (fun _ _ => [fun _ => None]) p).
     eexists (IdMap.mapi (fun _ _ => [fun _ => None]) p).
+    eexists (IdMap.mapi (fun _ _ => [fun _ => None]) p).
     eexists (IdMap.mapi (fun _ _ => [bot]) p).
     eexists (IdMap.mapi (fun _ _ => [bot]) p).
-    eexists (Execution.mk (IdMap.mapi (fun _ _ => _) p) bot bot bot bot bot bot).
+    eexists (Execution.mk (IdMap.mapi (fun _ _ => _) p) bot bot bot bot bot bot bot).
     eexists (@Valid.mk_pre_ex _ _ (IdMap.mapi (fun tid stmts => AExecUnit.mk (State.init stmts) ALocal.init) p)  _ _ _ _ _ _).
     hexploit Machine.rtc_promise_step_spec; eauto. s. intro X.
     s. splits; cycle 1.
@@ -351,12 +377,12 @@ Proof.
   generalize (SIM tid). intro Y. inv Y; [congr|]. rewrite TRS in H0. inv H0.
   hexploit sim_trace_last; eauto. i. des. subst. simplify.
   exploit promising_pf_sim_step; eauto.
-  { inv REL6; eauto. s.
+  { inv REL7; eauto. s.
     unfold Machine.init_with_promises in FIND0. ss.
     rewrite IdMap.mapi_spec, STMT in *. inv FIND0.
     apply sim_state_weak_init.
   }
-  { inv REL6; eauto. s.
+  { inv REL7; eauto. s.
     unfold Machine.init_with_promises in FIND0. ss.
     rewrite IdMap.mapi_spec, STMT in *. inv FIND0.
     auto.
@@ -368,9 +394,10 @@ Proof.
   eexists (IdMap.add tid _ atrs).
   eexists (IdMap.add tid _ ws).
   eexists (IdMap.add tid _ rs).
+  eexists (IdMap.add tid _ fs).
   eexists (IdMap.add tid _ covs).
   eexists (IdMap.add tid _ vexts).
-  eexists (Execution.mk _ _ _ _ _ _ _).
+  eexists (Execution.mk _ _ _ _ _ _ _ _).
   eexists (@Valid.mk_pre_ex _ _ (IdMap.add tid _ PRE.(Valid.aeus))  _ _ _ _ _ _).
   s. splits; cycle 1.
   - i. rewrite ? IdMap.add_spec. condtac; eauto.
@@ -382,28 +409,29 @@ all: ss.
 1: { ii. generalize (PRE.(Valid.AEUS) id). intro X.
      rewrite IdMap.add_spec. condtac; ss. inversion e0. subst. clear e0 X0.
      generalize (ATR tid). rewrite <- H. intro Y. inv Y. des. inv REL.
-     rewrite <- H6 in X. inv X. econs. etrans; eauto.
+     rewrite <- H7 in X. inv X. econs. etrans; eauto.
 }
-3: { funext. i. funext. i. propext. econs; ss. i. inv H.
+4: { funext. i. funext. i. propext. econs; ss. i. inv H.
      rewrite IdMap.map_spec, IdMap.mapi_spec in RELS. destruct (IdMap.find tid p); ss.
      inv RELS. inv REL. ss.
 }
-3: { funext. i. funext. i. propext. econs; ss. i. inv H.
+4: { funext. i. funext. i. propext. econs; ss. i. inv H.
      rewrite IdMap.map_spec, IdMap.mapi_spec in RELS. destruct (IdMap.find tid p); ss.
      inv RELS. inv REL. ss.
 }
-3: { funext. i. funext. i. propext. econs; ss. i. inv H.
+4: { funext. i. funext. i. propext. econs; ss. i. inv H.
      rewrite IdMap.map_spec, IdMap.mapi_spec in RELS. destruct (IdMap.find tid p); ss.
      inv RELS. inv REL. ss.
 }
-3: { funext. i. funext. i. propext. econs; ss. i. inv H.
+4: { funext. i. funext. i. propext. econs; ss. i. inv H.
      rewrite IdMap.map_spec, IdMap.mapi_spec in RELS. destruct (IdMap.find tid p); ss.
      inv RELS. inv REL. ss.
 }
-4: { ii. rewrite IdMap.mapi_spec. destruct (IdMap.find id p); ss. econs. refl. }
-3: { unfold IdMap.map. rewrite IdMap.mapi_mapi. f_equal. }
+5: { ii. rewrite IdMap.mapi_spec. destruct (IdMap.find id p); ss. econs. refl. }
+4: { unfold IdMap.map. rewrite IdMap.mapi_mapi. f_equal. }
 1: { apply bot. (* it's ex's co. *) }
 1: { apply bot. (* it's ex's rf. *) }
+1: { apply bot. (* it's ex's pf. *) }
 Qed.
 
 Inductive sim_th
@@ -412,6 +440,7 @@ Inductive sim_th
           (aeu:AExecUnit.t)
           (w: nat -> option (Loc.t * Time.t))
           (r: nat -> option (Loc.t * Time.t))
+          (f: nat -> option (Loc.t * Time.t))
           (cov: nat -> Time.t)
           (vext: nat -> Time.t): Prop := mk {
   WPROP1:
@@ -456,12 +485,29 @@ Inductive sim_th
       List.nth_error aeu.(AExecUnit.local).(ALocal.labels) eid = Some (Label.read ex ord loc val) /\
       __guard__ ((ts = Time.bot /\ val = Val.default) \/
                  Memory.get_msg ts mem = Some (Msg.mk loc val tid'));
+  FPROP1:
+    forall eid loc
+      (GET: List.nth_error aeu.(AExecUnit.local).(ALocal.labels) eid = Some (Label.flushopt loc)),
+    exists ts tid' val,
+      f eid = Some (loc, ts) /\
+      <<FLUSH_TS_SPEC:
+          __guard__ ((ts = Time.bot /\ val = Val.default) \/
+          Memory.get_msg ts mem = Some (Msg.mk loc val tid')) >>;
+  FPROP2:
+    forall eid loc ts (GET: f eid = Some (loc, ts)),
+    cov eid = ts /\
+    Time.le ts (vext eid) /\
+    exists val tid',
+      List.nth_error aeu.(AExecUnit.local).(ALocal.labels) eid = Some (Label.flushopt loc) /\
+      <<FLUSH_TS_SPEC:
+          __guard__ ((ts = Time.bot /\ val = Val.default) \/
+          Memory.get_msg ts mem = Some (Msg.mk loc val tid'))>>;
   COVPROP:
     forall eid (COV: cov eid > 0),
-      AExecUnit.label_is aeu.(AExecUnit.local).(ALocal.labels) Label.is_access eid;
+      AExecUnit.label_is aeu.(AExecUnit.local).(ALocal.labels) Label.is_access_persist eid;
   VEXTPROP:
     forall eid (VEXT: vext eid > 0),
-      AExecUnit.label_is aeu.(AExecUnit.local).(ALocal.labels) Label.is_access eid;
+      AExecUnit.label_is aeu.(AExecUnit.local).(ALocal.labels) Label.is_access_persist eid;
 
   PO: forall iid1 iid2 label1 label2
      (PO: iid1 < iid2)
@@ -485,13 +531,15 @@ Lemma sim_trace_sim_state_weak
       atr aeu atr'
       wl w wl'
       rl r rl'
+      fl f fl'
       covl cov covl'
       vextl vext vextl'
-      (SIM: sim_trace p mem tid tr atr wl rl covl vextl)
+      (SIM: sim_trace p mem tid tr atr wl rl fl covl vextl)
       (EU: tr = eu :: tr')
       (AEU: atr = aeu :: atr')
       (RL: rl = r :: rl')
       (WL: wl = w :: wl')
+      (FL: fl = f :: fl')
       (COV: covl = cov :: covl')
       (VEXT: vextl = vext :: vextl'):
   sim_state_weak eu.(ExecUnit.state) aeu.(AExecUnit.state).
@@ -507,22 +555,26 @@ Lemma sim_trace_sim_th
       atr aeu atr'
       wl w wl'
       rl r rl'
+      fl f fl'
       covl cov covl'
       vextl vext vextl'
-      (SIM: sim_trace p mem tid tr atr wl rl covl vextl)
+      (SIM: sim_trace p mem tid tr atr wl rl fl covl vextl)
       (EU: tr = eu :: tr')
       (AEU: atr = aeu :: atr')
       (RL: rl = r :: rl')
       (WL: wl = w :: wl')
+      (FL: fl = f :: fl')
       (COV: covl = cov :: covl')
       (VEXT: vextl = vext :: vextl'):
-  sim_th p mem tid eu aeu w r cov vext.
+  sim_th p mem tid eu aeu w r f cov vext.
 Proof.
-  revert r rl' w wl' eu tr' aeu atr' cov covl' vext vextl' RL WL EU AEU COV VEXT. induction SIM.
+  revert f fl' r rl' w wl' eu tr' aeu atr' cov covl' vext vextl' FL RL WL EU AEU COV VEXT. induction SIM.
   { i. simplify. ss. econs; ss.
     - rewrite IdMap.mapi_spec, STMT in FIND. inv FIND. s. i.
       left. splits; ss. destruct ts; ss.
       eapply Promises.promises_from_mem_lookup. eauto.
+    - rewrite IdMap.mapi_spec, STMT in FIND. inv FIND. s. i.
+      destruct eid; ss.
     - rewrite IdMap.mapi_spec, STMT in FIND. inv FIND. s. i.
       destruct eid; ss.
     - rewrite IdMap.mapi_spec, STMT in FIND. inv FIND. s. i.
@@ -615,6 +667,14 @@ Proof.
         * rewrite fun_add_spec. des_ifs; eauto.
           inv e. etrans; eauto. ss. apply join_l.
         * eapply nth_error_app_mon. eauto.
+    - i. des. exploit IH.(FPROP1); eauto.
+      apply nth_error_snoc_inv in GET. des; ss.
+    - i. exploit IH.(FPROP2); eauto. s. i. des. des_ifs; cycle 1.
+      { esplits; eauto. eapply nth_error_app_mon in x2. eauto. }
+      exfalso. apply Nat.eqb_eq in Heq. subst.
+      unfold ALocal.next_eid in *.
+      assert (H: List.nth_error (ALocal.labels alc1) (length (ALocal.labels alc1)) <> None) by (ii; congr).
+      apply List.nth_error_Some in H. lia.
     - unfold ALocal.next_eid in *. s. i. des_ifs.
       { apply Nat.eqb_eq in Heq. subst. econs; eauto.
         - rewrite List.nth_error_app2, Nat.sub_diag; [|refl]. ss.
@@ -738,6 +798,14 @@ Proof.
       * rewrite fun_add_spec. des_ifs; eauto. inv e. etrans; eauto.
         inv WRITABLE. apply Nat.lt_le_incl. ss.
       * eapply nth_error_app_mon. eauto.
+    - i. des. exploit IH.(FPROP1); eauto.
+      apply nth_error_snoc_inv in GET. des; ss.
+    - i. exploit IH.(FPROP2); eauto. s. i. des. des_ifs; cycle 1.
+      { esplits; eauto. eapply nth_error_app_mon in x2. eauto. }
+      exfalso. apply Nat.eqb_eq in Heq. subst.
+      unfold ALocal.next_eid in *.
+      assert (H: List.nth_error (ALocal.labels alc1) (length (ALocal.labels alc1)) <> None) by (ii; congr).
+      apply List.nth_error_Some in H. lia.
     - unfold ALocal.next_eid in *. s. i. des_ifs.
       { apply Nat.eqb_eq in Heq. subst. econs; eauto.
         - rewrite List.nth_error_app2, Nat.sub_diag; [|refl]. ss.
@@ -797,6 +865,10 @@ Proof.
         apply nth_error_snoc_inv in GET. des; eauto. congr.
       - i. exploit IH.(RPROP2); eauto. s. i. des. esplits; eauto.
         eapply nth_error_app_mon. eauto.
+      - i. exploit IH.(FPROP1); eauto.
+        apply nth_error_snoc_inv in GET. des; eauto. congr.
+      - i. exploit IH.(FPROP2); eauto. s. i. des. esplits; eauto.
+        eapply nth_error_app_mon. eauto.
       - i. apply AExecUnit.label_is_mon. eapply IH.(COVPROP); eauto.
       - i. apply AExecUnit.label_is_mon. eapply IH.(VEXTPROP); eauto.
       - i. apply nth_error_snoc_inv in LABEL1. des; cycle 1.
@@ -818,6 +890,10 @@ Proof.
         apply nth_error_snoc_inv in GET. des; eauto. congr.
       - i. exploit IH.(RPROP2); eauto. s. i. des. esplits; eauto.
         eapply nth_error_app_mon. eauto.
+      - i. exploit IH.(FPROP1); eauto.
+        apply nth_error_snoc_inv in GET. des; eauto. congr.
+      - i. exploit IH.(FPROP2); eauto. s. i. des. esplits; eauto.
+        eapply nth_error_app_mon. eauto.
       - i. apply AExecUnit.label_is_mon. eapply IH.(COVPROP); eauto.
       - i. apply AExecUnit.label_is_mon. eapply IH.(VEXTPROP); eauto.
       - i. apply nth_error_snoc_inv in LABEL1. des; cycle 1.
@@ -838,6 +914,10 @@ Proof.
       - i. exploit IH.(RPROP1); eauto.
         apply nth_error_snoc_inv in GET. des; eauto. congr.
       - i. exploit IH.(RPROP2); eauto. s. i. des. esplits; eauto.
+        eapply nth_error_app_mon. eauto.
+      - i. exploit IH.(FPROP1); eauto.
+        apply nth_error_snoc_inv in GET. des; eauto. congr.
+      - i. exploit IH.(FPROP2); eauto. s. i. des. esplits; eauto.
         eapply nth_error_app_mon. eauto.
       - i. apply AExecUnit.label_is_mon. eapply IH.(COVPROP); eauto.
       - i. apply AExecUnit.label_is_mon. eapply IH.(VEXTPROP); eauto.
@@ -862,6 +942,10 @@ Proof.
       apply nth_error_snoc_inv in GET. des; eauto. congr.
     - i. exploit IH.(RPROP2); eauto. s. i. des. esplits; eauto.
       eapply nth_error_app_mon. eauto.
+    - i. exploit IH.(FPROP1); eauto.
+      apply nth_error_snoc_inv in GET. des; eauto. congr.
+    - i. exploit IH.(FPROP2); eauto. s. i. des. esplits; eauto.
+      eapply nth_error_app_mon. eauto.
     - i. apply AExecUnit.label_is_mon. eapply IH.(COVPROP); eauto.
     - i. apply AExecUnit.label_is_mon. eapply IH.(VEXTPROP); eauto.
     - i. apply nth_error_snoc_inv in LABEL1. des; cycle 1.
@@ -877,13 +961,25 @@ Proof.
       eapply nth_error_app_mon. eauto.
     - i. exploit IH.(WPROP2); eauto.
       apply nth_error_snoc_inv in GET. des; eauto. congr.
-    - i. exploit IH.(WPROP3); eauto. s. i. des. esplits; eauto.
-      eapply nth_error_app_mon. eauto.
+    - i. exploit IH.(WPROP3); eauto. s. i. des. des_ifs.
+      { exfalso. apply Nat.eqb_eq in Heq. subst.
+        unfold ALocal.next_eid in *.
+        assert (H: List.nth_error (ALocal.labels alc1) (length (ALocal.labels alc1)) <> None) by (ii; congr).
+        apply List.nth_error_Some in H. lia.
+      }
+      esplits; eauto. eapply nth_error_app_mon. eauto.
     - eapply IH.(WPROP4).
     - i. exploit IH.(RPROP1); eauto.
       apply nth_error_snoc_inv in GET. des; eauto. congr.
     - i. exploit IH.(RPROP2); eauto. s. i. des. esplits; eauto.
-      eapply nth_error_app_mon. eauto.
+      + des_ifs.
+        exfalso. apply Nat.eqb_eq in Heq. subst.
+        unfold ALocal.next_eid in *.
+        assert (H: List.nth_error (ALocal.labels alc1) (length (ALocal.labels alc1)) <> None) by (ii; congr).
+        apply List.nth_error_Some in H. lia.
+      + eapply nth_error_app_mon. eauto.
+    - admit.
+    - admit.
     - i. apply AExecUnit.label_is_mon. eapply IH.(COVPROP); eauto.
     - i. apply AExecUnit.label_is_mon. eapply IH.(VEXTPROP); eauto.
     - i. apply nth_error_snoc_inv in LABEL1. des; cycle 1.
